src/program_proof/tulip/paxos/invariance/commit.v
@@ -14,14 +14,16 @@ Section commit.
     by iApply (nodes_inv_safe_ledger_in_impl_chosen_in with "Hsafe Hinv").
   Qed.
 
-  Lemma paxos_inv_commit γ nids logi' :
-    safe_ledger γ nids logi' -∗
-    paxos_inv γ nids ==∗
-    paxos_inv γ nids ∗
-    is_internal_log_lb γ logi'.
+  Lemma safe_ledger_log_impl_prefix γ nids v v' :
+    safe_ledger γ nids v' -∗
+    own_log_half γ v -∗
+    paxos_inv γ nids -∗
+    ⌜prefix v v' ∨ prefix v' v⌝.
   Proof.
-    iIntros "#Hsafe Hinv".
+    iIntros "#Hsafe Hloguser Hinv".
     iNamed "Hinv".
+    (* Agreement on the log content. *)
+    iDestruct (log_agree with "Hloguser Hlog") as %->.
     (* Extract past decisions and accepted proposals from the node invariant. *)
     iDestruct (nodes_inv_extract_ds_psa with "Hnodes") as (dss bs) "[Hnodes Hpds]".
     iDestruct (big_sepM2_dom with "Hpds") as %Hdompds.
@@ -40,24 +42,59 @@ Section commit.
     (* Finally, derive [consistency bs]. *)
     pose proof (vlb_vub_vbp_vp_impl_consistency _ _ _ Hvlb Hvub Hvbp Hvp) as Hcst.
     (* Now, derive [chosen bs logi] and [chosen bs logi']. *)
-    iDestruct (nodes_inv_safe_ledger_impl_chosen _ _ bs with "Hsafelogi [Hpds]") as %Hchosen.
+    iDestruct (nodes_inv_safe_ledger_impl_chosen _ _ bs with "Hsafelog [Hpds]") as %Hchosen.
     { apply Hdombs. }
     { by iApply nodes_inv_ds_psa_impl_nodes_inv_psa. }
     iDestruct (nodes_inv_safe_ledger_impl_chosen _ _ bs with "Hsafe [Hpds]") as %Hchosen'.
     { apply Hdombs. }
     { by iApply nodes_inv_ds_psa_impl_nodes_inv_psa. }
     (* Derive [prefix logi logi' ∨ prefix logi' logi]. *)
-    specialize (Hcst _ _ Hchosen Hchosen').
-    (* Merge [node_inv_ds_psa] back. *)
-    iDestruct (nodes_inv_merge_ds_psa with "Hnodes Hpds") as "Hnodes".
-    destruct Hcst as [Hge | Hle]; last first.
-    { (* Case: The old log is at least as long as the new log. Simply extract a witness. *)
-      iDestruct (internal_log_witness logi' with "Hlogi") as "#Hlb"; first apply Hle.
-      by iFrame "∗ # %".
+    by specialize (Hcst _ _ Hchosen Hchosen').
+  Qed.
+
+  Lemma paxos_inv_commit {γ nids nid vcli vnode} vsafe :
+    nid ∈ nids ->
+    prefix vsafe vnode ->
+    safe_ledger γ nids vsafe -∗
+    own_log_half γ vcli -∗
+    own_node_ledger_half γ nid vnode -∗
+    paxos_inv γ nids ==∗
+    (∃ vcli', own_log_half γ vcli' ∧ ⌜prefix vsafe vcli'⌝) ∗
+    own_node_ledger_half γ nid vnode ∗
+    paxos_inv γ nids.
+  Proof.
+    iIntros (Hnid Hprefix) "#Hsafe Hlogcli HlognX Hinv".
+    iDestruct (safe_ledger_log_impl_prefix with "Hsafe Hlogcli Hinv") as %Horprefix.
+    destruct Horprefix as [Hext | Hnoext]; last first.
+    { (* Case: The global log is longer than the committed log on [nid]. No update required. *)
+      by iFrame.
     }
-    (* Case: The new log is at least as long as the old log. Update the log. *)
-    iMod (internal_log_update with "Hlogi") as "Hlogi"; first apply Hge.
-    iDestruct (internal_log_witness logi' with "Hlogi") as "#Hlb"; first done.
+    (* Case: The global log is shorted. Extend it to [vsafe]. *)
+    iNamed "Hinv".
+    iDestruct (log_agree with "Hlogcli Hlog") as %->.
+    iAssert (⌜cpool_subsume_log vsafe cpool⌝)%I as %Hsubsume.
+    { rewrite -Hdomtermlm elem_of_dom in Hnid.
+      destruct Hnid as [terml Hterml].
+      iDestruct (big_sepM_lookup with "Hnodes") as "Hnode"; first apply Hterml.
+      iNamed "Hnode".
+      iDestruct (node_ledger_agree with "HlognX Hlogn") as %->.
+      iDestruct (accepted_proposal_lookup with "Hacpt Hpsa") as %Hvnode.
+      iDestruct (big_sepM_lookup with "Hpsaubs") as (vub1) "[#Hvub1 %Hprefix1]"; first apply Hvnode.
+      iDestruct (proposals_prefix with "Hvub1 Hps") as (vub2) "[%Hvub2 %Hprefix2]".
+      assert (Hvsafe : prefix vsafe vub2).
+      { trans vnode; first apply Hprefix.
+        trans vub1; [apply Hprefix1 | apply Hprefix2].
+      }
+      iDestruct (big_sepM_lookup with "Hsubsume") as "Hpcmds"; first apply Hvub2.
+      rewrite /cpool_subsume_log Forall_forall.
+      iIntros (c Hc).
+      pose proof (elem_of_prefix _ _ _ Hc Hvsafe) as Hc'.
+      iDestruct (big_sepL_elem_of with "Hpcmds") as "Hc"; first apply Hc'.
+      iApply (cpool_lookup with "Hc Hcpool").
+    }
+    iMod (log_update with "Hlogcli Hlog Hcpool") as "(Hlogcli & Hlog & Hcpool)".
+    { apply Hsubsume. }
+    { apply Hext. }
     by iFrame "∗ # %".
   Qed.
 
