src/program_proof/tulip/paxos/invariance/extend.v
@@ -3,27 +3,109 @@ From Perennial.program_proof.tulip.paxos Require Import prelude.
 Section extend.
   Context `{!paxos_ghostG Σ}.
 
-  Lemma paxos_inv_extend γ nids term logn logn' :
-    prefix logn logn' ->
-    own_proposal γ term logn -∗
-    paxos_inv γ nids ==∗
-    own_proposal γ term logn' ∗
-    paxos_inv γ nids.
+  Lemma node_inv_extend {γ nid term v} v' :
+    prefix v v' ->
+    is_proposal_lb γ term v' -∗
+    own_current_term_half γ nid term -∗
+    own_node_ledger_half γ nid v -∗
+    node_inv γ nid term ==∗
+    own_current_term_half γ nid term ∗
+    own_node_ledger_half γ nid v' ∗
+    node_inv γ nid term ∗
+    is_accepted_proposal_lb γ nid term v'.
   Proof.
-    iIntros (Hprefix) "Hp Hinv".
-    iNamed "Hinv".
-    iDestruct (proposal_lookup with "Hp Hps") as %Hlogn.
-    (* Extend the growing proposal to [logn'] and extract a witness. *)
-    iMod (proposal_update logn' with "Hp Hps") as "[Hp Hps]"; first apply Hprefix.
+    iIntros (Hprefix) "#Hpslb HtermcX HlognX Hnode".
+    iNamed "Hnode".
+    (* Agreements. *)
+    iDestruct (current_term_agree with "HtermcX Htermc") as %->.
+    iDestruct (node_ledger_agree with "HlognX Hlogn") as %->.
+    (* Update the node-local ledger. *)
+    iMod (node_ledger_update v' with "HlognX Hlogn") as "[HlognX Hlogn]".
+    iDestruct (accepted_proposal_lookup with "Hacpt Hpsa") as %Hv.
+    (* Update the accepted ledger at [term]. *)
+    iMod (accepted_proposal_update v' with "Hacpt Hpsa") as "[Hacpt Hpsa]".
+    { apply Hprefix. }
+    iDestruct (accepted_proposal_witness with "Hacpt") as "#Hacptlb".
     iFrame "∗ # %".
+    iModIntro.
+    iSplit.
+    { (* Re-establish [prefix_base_ledger]. *)
+      iDestruct (big_sepM_lookup with "Hpsalbs") as (vlb) "[#Hlb %Hprefixv]"; first apply Hv.
+      iApply big_sepM_insert_2; last done.
+      iFrame "Hlb".
+      iPureIntro.
+      by trans v.
+    }
+    iSplit.
+    { (* Re-establish [prefix_growing_ledger]. *)
+      iApply big_sepM_insert_2; last done.
+      by iFrame "Hpslb".
+    }
+    iPureIntro.
+    split.
+    { (* Re-establish [fixed_proposals]. *)
+      intros t d Hd.
+      specialize (Hfixed _ _ Hd).
+      destruct (decide (t = term)) as [-> | Hne]; last by rewrite lookup_insert_ne.
+      exfalso.
+      apply lookup_lt_Some in Hd.
+      clear -Hd Hlends. lia.
+    }
+    { (* Re-establish [free_terms_after]. *)
+      apply elem_of_dom_2 in Hv.
+      rewrite dom_insert_L.
+      by replace (_ ∪ dom psa) with (dom psa) by set_solver.
+    }
+  Qed.
+
+  Lemma paxos_inv_extend {γ nids nid term v} vapp :
+    let v' := v ++ vapp in
+    nid ∈ nids ->
+    proposed_cmds γ vapp -∗
+    own_proposal γ term v -∗
+    own_current_term_half γ nid term -∗
+    own_ledger_term_half γ nid term -∗
+    own_node_ledger_half γ nid v -∗
+    paxos_inv γ nids ==∗
+    own_proposal γ term v' ∗
+    own_current_term_half γ nid term ∗
+    own_ledger_term_half γ nid term ∗
+    own_node_ledger_half γ nid v' ∗
+    paxos_inv γ nids ∗
+    is_accepted_proposal_lb γ nid term v'.
+  Proof.
+    iIntros (v' Hnid) "#Hpcs Hp Htermc Hterml Hlogn Hinv".
+    iNamed "Hinv".
+    iDestruct (proposal_lookup with "Hp Hps") as %Hv.
+    (* Re-establish [proposed_cmds] on the new log [v ++ vapp]. *)
+    iAssert (proposed_cmds γ (v ++ vapp))%I as "Hsubsume'".
+    { iDestruct (big_sepM_lookup with "Hsubsume") as "Hpcsv"; first apply Hv.
+      iFrame "#".
+    }
+    (* Extend the growing proposal to [v'] and extract a witness. *)
+    iMod (proposal_update (v ++ vapp) with "Hp Hps") as "[Hp Hps]"; first by apply prefix_app_r.
+    iDestruct (proposal_witness with "Hp") as "#Hplb".
+    (* Update the node-local ledger. *)
+    rewrite -Hdomtermlm elem_of_dom in Hnid.
+    destruct Hnid as [terml Hterml].
+    iDestruct (big_sepM_lookup_acc _ _ nid with "Hnodes") as "[Hnode HnodesC]".
+    { apply Hterml. }
+    iDestruct (own_ledger_term_node_inv_terml_eq with "Hterml Hnode") as %->.
+    iMod (node_inv_extend v' with "Hplb Htermc Hlogn Hnode")
+      as "(Htermc & Hlogn & Hnode & #Hacpted)".
+    { by apply prefix_app_r. }
+    iDestruct ("HnodesC" with "Hnode") as "Hnodes".
+    iFrame "∗ # %".
+    iModIntro.
+    iSplit; first by iApply big_sepM_insert_2.
     iPureIntro.
     intros t.
     destruct (decide (t = term)) as [-> | Hne]; last by rewrite lookup_insert_ne.
     rewrite lookup_insert.
     specialize (Hvp term).
-    destruct (psb !! term) as [loglb |] eqn:Hloglb; rewrite Hlogn Hloglb /= in Hvp; last done.
+    destruct (psb !! term) as [loglb |] eqn:Hloglb; rewrite Hv Hloglb /= in Hvp; last done.
     rewrite Hloglb /=.
-    by trans logn.
+    by trans v; last apply prefix_app_r.
   Qed.
 
 End extend.
